src/ePlugin.mli
@@ -8,3 +8,4 @@ val implement : ?exn:reference -> Id.t -> Constrexpr.constr_expr -> unit
 val pimplement : ?exn:reference -> reference -> unit
 
 val wtranslate : ?exn:reference -> ?names:Id.t list -> reference -> unit
+val wimplement : ?exn:reference -> reference -> unit
