theories/Effects.v
@@ -43,3 +43,131 @@ match A with
 | pTypeVal _ A _ => A
 | pTypeErr _ e => True
 end.
+
+(******************************)
+(*** Test handling of sorts ***)
+(******************************)
+
+(*
+Module Test.
+Set Universe Polymorphism.
+Inductive sort@{i j} (E : Type@{i}) : Prop :=
+| sortType : forall (A : Type@{j}), (E -> A) -> sort E
+| sortProp : forall (A : Prop), (E -> A) -> sort E
+| sortErr : E -> sort E.
+Print sort.
+Definition type@{i j} (E: Type@{i}) : Type@{j}.
+Proof. exact (sort@{i j} E). Defined.
+
+Definition sTypeVal@{i j} (E: Type@{i}) (A: Type@{j}) (f: E -> A): type@{i j} E :=
+  sortType E A f. Print sTypeVal.
+Definition sTypeErr@{i j} (E: Type@{i}) (e: E): type@{i j} E :=
+  sortErr E e.
+
+Definition prop@{i} (E: Type@{i}) : Prop :=
+  sort@{i Set} E.
+Definition sPropVal@{i} (E: Type@{i}) (A: Prop) (f: E -> A): type@{i Set} E :=
+  sortType E A f. Print sPropVal.
+Definition sPropErr@{i j} (E: Type@{i}) (e: E): type@{i Set} E :=
+  sortErr E e.
+
+Definition sEl@{i j} {E : Type@{i}} (A : type@{i j} E) : Type@{j} :=
+match A with
+| sortType _ A _ => A
+| sortProp _ _ _ => any@{j}
+| sortErr _ _ => any@{j}
+end.
+
+Definition sErr@{i j} {E : Type@{i}} (A : sort@{i j} E) : E -> sEl@{i j} A :=
+match A return E -> sEl A with
+| sTypeVal _ _ e => e
+| sPropVal _ _ _ => fun _ => Any
+| sSortErr _ _ => fun _ => Any
+end.
+
+Definition sType@{i j k} {E : Type@{i}} : sort@{i k} E :=
+  sTypeVal E (sort@{i j} E) (sSortErr E).
+
+(** Prop related *)
+Definition spEl@{i} {E : Type@{i}} (A: sort@{i Set} E) : Prop:=
+match A with
+| sTypeVal _ _ _ => True
+| sPropVal _ A _ => A
+| sSortErr _ _ => True
+end.
+
+Definition spErr@{i j} {E : Type@{i}} (A : sort@{i Set} E) : E -> spEl@{i} A :=
+match A return E -> spEl A with
+| sTypeVal _ _ e => fun _ => I
+| sPropVal _ _ e => e
+| sSortErr _ _ => fun _ => I
+end.
+
+Definition sProp@{i j} {E : Type@{i}} : sort@{i j} E :=
+  sTypeVal E (sort@{i Set} E) (PropErr E). 
+
+End Test.
+*)
+
+(***************************)
+(** New handling of sorts **)
+(***************************)
+
+Module NewExc.
+Set Universe Polymorphism.
+Cumulative Inductive sort@{i j} (E : Type@{i}) : Type :=
+| sortType : forall (A : Type@{j}), (E -> A) -> sort E
+| sortProp : forall (A : Prop), (E -> A) -> sort E
+| sortErr : E -> sort E.
+
+Definition type@{i j} (E: Type@{i}) :=
+  sort@{i j} E.
+Definition sTypeVal@{i j} (E: Type@{i}) (A: Type@{j}) (f: E -> A): type@{i j} E :=
+  sortType E A f.
+Definition sTypeErr@{i j} (E: Type@{i}) (e: E): type@{i j} E :=
+  sortErr E e.
+
+Definition prop@{i} (E: Type@{i}) :=
+  sort@{i Set} E.
+Definition sPropVal@{i} (E: Type@{i}) (A: Prop) (f: E -> A): prop@{i} E :=
+  sortProp E A f.
+Definition sPropErr@{i} (E: Type@{i}) (e: E): prop@{i} E :=
+  sortErr E e.
+
+(** Type related *)
+Definition sEl@{i j} {E : Type@{i}} (A : type@{i j} E) : Type@{j} :=
+match A with
+| sortType _ A _ => A
+| sortProp _ _ _ => any@{j}
+| sortErr  _ _ => any@{j}
+end.
+
+Definition sErr@{i j} {E : Type@{i}} (A : type@{i j} E) : E -> sEl@{i j} A :=
+match A return E -> sEl A with
+| sortType _ _ e => e
+| sortProp _ _ _ => fun _ => Any
+| sortErr  _ _ => fun _ => Any
+end.
+
+Definition sType@{i j k} {E : Type@{i}} : type@{i k} E :=
+  sTypeVal E (type@{i j} E) (sTypeErr E).
+
+(** Prop related *)
+Definition spEl@{i} {E : Type@{i}} (A: prop@{i} E) : Prop:=
+match A with
+| sortType _ _ _ => True
+| sortProp _ A _ => A
+| sortErr  _ _ => True
+end.
+
+Definition spErr@{i j} {E : Type@{i}} (A : sort@{i Set} E) : E -> spEl@{i} A :=
+match A return E -> spEl A with
+| sortType _ _ e => fun _ => I
+| sortProp _ _ e => e
+| sortErr  _ _ => fun _ => I
+end.
+
+Definition sProp@{i j} {E : Type@{i}} : type@{i j} E :=
+  sTypeVal E (prop@{i} E) (sPropErr E).
+
+End NewExc.
